Hs/Translator/Lemmas/TypesSoundness.lean
@@ -11,16 +11,38 @@ import SystemFD.Metatheory.Inversion
 
 import Batteries.Lean.Except
 
-theorem is_type_spine_application (Γ : Ctx Term) (τh : Term) (τs : List Term) : ⊢ Γ ->
+theorem is_type_list_reverse (τs : List Term) :
+  (∀ τ ∈ τs, Term.IsType τ) -> ∀ τ ∈ τs.reverse, Term.IsType τ := by
+  intro h t h2
+  have lem : t ∈ τs := by simp at h2; assumption
+  replace h := h t lem
+  assumption
+
+
+theorem is_type_spine_application' (τh : Term) (τs : List Term) :
   τh.IsType ->
   (∀ τ ∈ τs, Term.IsType τ) ->
-  Term.IsType (Term.mk_ty_apps_rev τ τs.reverse) := by
-intro wf h1 h2
+  Term.IsType (τh.mk_kind_apps' τs) := by
+intro h1 h2; simp at *
+induction τs using List.foldr.induct <;> simp at *
+case _ => assumption
+case _ ih =>
+  cases h2; case _ h2a h2b =>
+  constructor;
+  replace ih := ih h2b; assumption
+  assumption
 
-sorry
 
-
-
+theorem is_type_spine_application (τh : Term) (τs : List Term) :
+  τh.IsType ->
+  (∀ τ ∈ τs, Term.IsType τ) ->
+  Term.IsType (τh.mk_kind_apps τs) := by
+intro h1 h2
+have lem := is_type_list_reverse τs h2
+unfold Term.mk_kind_apps
+apply is_type_spine_application'
+assumption
+assumption
 
 theorem compile_type_shape_soundness (Γ : Ctx Term) (k : Term) (τ : HsTerm) (τ' : Term): ⊢ Γ ->
  HsTerm.IsType τ ->
@@ -79,31 +101,48 @@ case _ sp idx _ tnfp _ _ _ _ =>
     simp at j5; cases j5; case _ j6 j5 =>
     cases j6; case _ j6 j7 =>
     have e := Term.eq_of_beq j6; cases e; clear j6
-    cases j3; case _ j3 j6 =>
+    cases j3; case _ exp_κ τ _ _ _ _ _ j3 j6 =>
     cases j6;
-    generalize zzh : κs.attach.zip sp.attach = zz at *
-    induction κs generalizing sp <;> simp at zzh
-    case _ =>
-      cases zzh
-      simp at j3; unfold pure at j3; unfold Applicative.toPure at j3;
-      unfold Monad.toApplicative at j3; unfold Except.instMonad at j3; simp at j3;
-      unfold Except.pure at j3; simp at j3; cases j3; simp; constructor
-    case _ κhd κtl _ _ =>
-      induction sp <;> simp at zzh
+    have lem1 := HsTerm.hs_type_neutral_form_is_type j1 tnfp
+    have lem2 := HsTerm.hs_is_type_neutral_form j1 tnfp
+    cases lem1; case _ lem1a =>
+    -- have κ_wf : κ.IsKind := by sorry
+    -- have lem3 := kind_shape_split_arrow κ_wf j4
+    -- cases lem3; case _ lem3a lem3b =>
+    rw[List.foldl_eq_foldr_reverse]
+    apply is_type_spine_application
+    case _ => constructor
+    case _ ih _ _ =>
+      intro sp_τ τ_in_sp
+      induction [], κ using Term.split_kind_arrow_aux.induct <;> simp at j4
+      sorry
+      -- have ih' := ih κs
       case _ =>
-        cases zzh
-        simp at j3; unfold pure at j3; unfold Applicative.toPure at j3;
-        unfold Monad.toApplicative at j3; unfold Except.instMonad at j3; simp at j3;
-        unfold Except.pure at j3; simp at j3; cases j3; simp; constructor
-      case _ sph sptl _ _ =>
-        rw[<-zzh] at j3; rw[<-List.mapM'_eq_mapM] at j3
-        simp at j3
-        unfold bind at j3; unfold Monad.toBind at j3; unfold Except.instMonad at j3; simp at j3
-        cases j3; case _ j3 =>
-        cases j3; case _ j3a j3b =>
-        simp at j3a; simp at j3b
-        unfold Except.map at j3b; split at j3b <;> simp at j3b
-        cases j3b; simp; sorry
+        cases j4.1; cases j4.2; simp at j3; cases j3; cases τ_in_sp
+
+    -- generalize zzh : κs.attach.zip sp.attach = zz at *
+    -- induction κs generalizing sp <;> simp at zzh
+    -- case _ =>
+    --   cases zzh
+    --   simp at j3; unfold pure at j3; unfold Applicative.toPure at j3;
+    --   unfold Monad.toApplicative at j3; unfold Except.instMonad at j3; simp at j3;
+    --   unfold Except.pure at j3; simp at j3; cases j3; simp; constructor
+    -- case _ κhd κtl _ _ =>
+    --   induction sp <;> simp at zzh
+    --   case _ =>
+    --     cases zzh
+    --     simp at j3; unfold pure at j3; unfold Applicative.toPure at j3;
+    --     unfold Monad.toApplicative at j3; unfold Except.instMonad at j3; simp at j3;
+    --     unfold Except.pure at j3; simp at j3; cases j3; simp; constructor
+    --   case _ sph sptl _ _ =>
+    --     rw[<-zzh] at j3; rw[<-List.mapM'_eq_mapM] at j3
+    --     simp at j3
+    --     unfold bind at j3; unfold Monad.toBind at j3; unfold Except.instMonad at j3; simp at j3
+    --     cases j3; case _ j3 =>
+    --     cases j3; case _ j3a j3b =>
+    --     simp at j3a; simp at j3b
+    --     unfold Except.map at j3b; split at j3b <;> simp at j3b
+    --     cases j3b; rw[List.foldl_eq_foldr_reverse]; sorry
 
 
 
